Auto/Lib/BinTree.lean
@@ -1,35 +1,309 @@
-import Auto.Lib.BinNat
+import Std.Data.Nat.Lemmas
+import Auto.Lib.Containers
+
+namespace Auto
+
+namespace Bin
+
+private theorem wfAux (n n' : Nat) : n = n' + 2 → n / 2 < n := by
+  intro H; apply Nat.div_lt_self
+  case hLtN =>
+    cases n;
+    contradiction;
+    apply Nat.succ_le_succ; apply Nat.zero_le
+  case hLtK => apply Nat.le_refl
+
+theorem inductionOn.{u}
+  {motive : Nat → Sort u} (x : Nat)
+  (ind : ∀ x, motive ((x + 2) / 2) → motive (x + 2))
+  (base₀ : motive 0) (base₁ : motive 1) : motive x :=
+  match h : x with
+  | 0 => base₀
+  | 1 => base₁
+  | x' + 2 => ind x' (inductionOn ((x' + 2) / 2) ind base₀ base₁)
+decreasing_by apply wfAux; rfl
+
+theorem induction.{u}
+  {motive : Nat → Sort u}
+  (ind : ∀ x, motive ((x + 2) / 2) → motive (x + 2))
+  (base₀ : motive 0) (base₁ : motive 1) : ∀ x, motive x :=
+  fun x => inductionOn x ind base₀ base₁
+
+end Bin
 
 inductive BinTree (α : Sort _) where
   | leaf : BinTree α
-  | node : BinTree α → α → BinTree α → BinTree α
+  | node : BinTree α → Option α → BinTree α → BinTree α
 
-structure BinList (α : Sort _) where
-  zero : α
-  pos  : BinTree α
+namespace BinTree
 
-def BinTree.val (bt : BinTree α) (default : α) :=
+instance : Inhabited (BinTree α) where
+  default := .leaf
+
+def val? (bt : BinTree α) : Option α :=
   match bt with
-  | .leaf => default
+  | .leaf => .none
   | .node _ x _ => x
 
-def BinTree.left (bt : BinTree α) :=
+def valD (bt : BinTree α) (default : α) :=
+  bt.val?.getD default
+
+def left! (bt : BinTree α) :=
   match bt with
-  | .leaf => BinTree.leaf
+  | .leaf => leaf
   | .node l _ _ => l
 
-def BinTree.right (bt : BinTree α) :=
+def right! (bt : BinTree α) :=
   match bt with
-  | .leaf => BinTree.leaf
+  | .leaf => leaf
   | .node _ _ r => r
 
-def BinTree.get (bt : BinTree α) (default : α) (bs : Pos) :=
-  match bs with
-  | .xH => bt.val default
-  | .xO bs' => BinTree.get bt.left default bs'
-  | .xI bs' => BinTree.get bt.right default bs'
+def get?WF (bt : BinTree α) (n : Nat) : Option α :=
+  match h : n with
+  | 0 => .none
+  | 1 => bt.val?
+  | _ + 2 =>
+    match Nat.mod n 2 with
+    | 0 => get?WF bt.left! (Nat.div n 2)
+    | _ + 1 => get?WF bt.right! (Nat.div n 2)
+termination_by get?WF bt n => n
+decreasing_by apply Bin.wfAux; assumption
+
+theorem get?WF.succSucc (bt : BinTree α) (n : Nat) :
+  get?WF bt (n + 2) = 
+    match Nat.mod (n + 2) 2 with
+    | 0 => get?WF bt.left! (Nat.div (n + 2) 2)
+    | _ + 1 => get?WF bt.right! (Nat.div (n + 2) 2) := rfl
+
+def get?Aux (bt : BinTree α) (n rd : Nat) : Option α :=
+  match rd with
+  | 0 => .none
+  | .succ rd' =>
+    match n with
+    | 0 => .none
+    | 1 => bt.val?
+    | _ + 2 =>
+      match Nat.mod n 2 with
+      | 0 => get?Aux bt.left! (Nat.div n 2) rd'
+      | _ + 1 => get?Aux bt.right! (Nat.div n 2) rd'
+
+theorem get?Aux.equiv (bt : BinTree α) (n rd : Nat) :
+  rd ≥ n → get?Aux bt n rd = get?WF bt n := by
+  revert n bt; induction rd <;> intros bt n H
+  case zero =>
+    have hzero : n = 0 := Nat.eq_zero_of_le_zero H
+    rw [hzero]; rfl
+  case succ rd' IH =>
+    dsimp [get?Aux]
+    match n with
+    | 0 => rfl
+    | 1 => rfl
+    | n' + 2 =>
+      dsimp;
+      rw [get?WF.succSucc];
+      have heq' : Nat.mod (n' + 2) 2 = n' % 2 := by
+        suffices (n' + 2) % 2 = n' % 2 by exact this
+        rw [Nat.add_mod_right]
+      have heqDiv : Nat.div (n' + 2) 2 = Nat.succ (n' / 2) := by
+        suffices (n' + 2) / 2 = Nat.succ (n' / 2) by exact this
+        rw [Nat.add_div_right]; simp
+      rw [heq', heqDiv];
+      have hge : rd' ≥ Nat.succ (n' / 2) := by
+        apply Nat.le_trans (m:=.succ n');
+        apply Nat.succ_le_succ; apply Nat.div_le_self
+        apply (Nat.le_of_succ_le_succ H)
+      rw [IH (left! bt), IH (right! bt)] <;> assumption
+
+def get? (bt : BinTree α) (n : Nat) : Option α :=
+  get?Aux bt n n
+
+theorem get?.equiv (bt : BinTree α) (n : Nat) :
+  get? bt n = get?WF bt n :=
+  get?Aux.equiv _ _ n .refl
+
+theorem get?.succSucc (bt : BinTree α) (n : Nat) :
+  get? bt (n + 2) = 
+    match (n + 2) % 2 with
+    | 0 => get? bt.left! ((n + 2) / 2)
+    | _ + 1 => get? bt.right! ((n + 2) / 2) := by
+  rw [get?.equiv bt, get?.equiv bt.left!, get?.equiv bt.right!]
+  apply get?WF.succSucc
+
+def insertWF (bt : BinTree α) (n : Nat) (x : α) : BinTree α :=
+  match h : n with
+  | 0 => bt
+  | 1 =>
+    match bt with
+    | .leaf => .node .leaf x .leaf
+    | .node l _ r => .node l x r
+  | _ + 2 =>
+    match Nat.mod n 2 with
+    | 0 =>
+      match bt with
+      | .leaf => .node (insertWF .leaf (Nat.div n 2) x) .none .leaf
+      | .node l v r => .node (insertWF l (Nat.div n 2) x) v r
+    | _ + 1 =>
+      match bt with
+      | .leaf => .node .leaf .none (insertWF .leaf (Nat.div n 2) x)
+      | .node l v r => .node l v (insertWF r (Nat.div n 2) x)
+termination_by insertWF bt n x => n
+decreasing_by rw [← h]; apply Bin.wfAux; assumption
+
+theorem insertWF.succSucc (bt : BinTree α) (n : Nat) (x : α) :
+  insertWF bt (n + 2) x = 
+    match Nat.mod (n + 2) 2 with
+    | 0 =>
+      match bt with
+      | .leaf => .node (insertWF .leaf (Nat.div (n + 2) 2) x) .none .leaf
+      | .node l v r => .node (insertWF l (Nat.div (n + 2) 2) x) v r
+    | _ + 1 =>
+      match bt with
+      | .leaf => .node .leaf .none (insertWF .leaf (Nat.div (n + 2) 2) x)
+      | .node l v r => .node l v (insertWF r (Nat.div (n + 2) 2) x) := rfl
+
+def insertAux (bt : BinTree α) (n : Nat) (x : α) (rd : Nat) : BinTree α :=
+  match rd with
+  | 0 => bt
+  | .succ rd' =>
+    match h : n with
+    | 0 => bt
+    | 1 =>
+      match bt with
+      | .leaf => .node .leaf x .leaf
+      | .node l _ r => .node l x r
+    | _ + 2 =>
+      match Nat.mod n 2 with
+      | 0 =>
+        match bt with
+        | .leaf => .node (insertAux .leaf (Nat.div n 2) x rd') .none .leaf
+        | .node l v r => .node (insertAux l (Nat.div n 2) x rd') v r
+      | _ + 1 =>
+        match bt with
+        | .leaf => .node .leaf .none (insertAux .leaf (Nat.div n 2) x rd')
+        | .node l v r => .node l v (insertAux r (Nat.div n 2) x rd')
+
+theorem insertAux.equiv (bt : BinTree α) (n : Nat) (x : α) (rd : Nat) :
+  rd ≥ n → insertAux bt n x rd = insertWF bt n x := by
+  revert n bt; induction rd <;> intros bt n H
+  case zero =>
+    have hzero : n = 0 := Nat.eq_zero_of_le_zero H
+    rw [hzero]; rfl
+  case succ rd' IH =>
+    dsimp [get?Aux]
+    match n with
+    | 0 => rfl
+    | 1 => rfl
+    | n' + 2 =>
+      dsimp [insertAux];
+      rw [insertWF.succSucc];
+      have heq' : Nat.mod (n' + 2) 2 = n' % 2 := by
+        suffices (n' + 2) % 2 = n' % 2 by exact this
+        rw [Nat.add_mod_right]
+      have heqDiv : Nat.div (n' + 2) 2 = Nat.succ (n' / 2) := by
+        suffices (n' + 2) / 2 = Nat.succ (n' / 2) by exact this
+        rw [Nat.add_div_right]; simp
+      rw [heq', heqDiv];
+      have hge : rd' ≥ Nat.succ (n' / 2) := by
+        apply Nat.le_trans (m:=.succ n');
+        apply Nat.succ_le_succ; apply Nat.div_le_self
+        apply (Nat.le_of_succ_le_succ H)
+      cases (n' % 2) <;> cases bt <;> dsimp <;> rw [IH] <;> assumption
+
+def insert (bt : BinTree α) (n : Nat) (x : α) := insertAux bt n x n
+
+theorem insert.equiv (bt : BinTree α) (n : Nat) (x : α) :
+  insert bt n x = insertWF bt n x :=
+  insertAux.equiv _ n x n .refl
+
+theorem insert.succSucc (bt : BinTree α) (n : Nat) (x : α) :
+  insert bt (n + 2) x = 
+    match (n + 2) % 2 with
+    | 0 =>
+      match bt with
+      | .leaf => .node (insert .leaf ((n + 2) / 2) x) .none .leaf
+      | .node l v r => .node (insert l ((n + 2) / 2) x) v r
+    | _ + 1 =>
+      match bt with
+      | .leaf => .node .leaf .none (insert .leaf ((n + 2) / 2) x)
+      | .node l v r => .node l v (insert r ((n + 2) / 2) x) := by
+  rw [insert.equiv bt, insertWF.succSucc]
+  rw [show Nat.mod (n + 2) 2 = (n + 2) % 2 by rfl]
+  rw [show Nat.div (n + 2) 2 = (n + 2) / 2 by rfl]
+  cases (n + 2) % 2 <;> cases bt <;> dsimp <;> rw [insert.equiv];
+
+theorem insert.correct₁ (bt : BinTree β) (n : Nat) (x : β) : n ≠ 0 → get? (insert bt n x) n = .some x := by
+  revert bt;
+  let motive := fun n => ∀ (bt : BinTree β), n ≠ 0 →
+    get? (insert bt n x) n = .some x
+  apply Bin.induction (motive := motive)
+  case base₀ => intros bt contra; contradiction
+  case base₁ => intros bt _; cases bt <;> rfl
+  case ind =>
+    intros n IH bt _
+    have hne' : (n + 2) / 2 ≠ 0 := by
+      rw [Nat.add_div_right _ (.step .refl)]; intro h; cases h
+    let IH' := fun bt => IH bt hne'
+    rw [get?.succSucc, insert.succSucc, left!, right!]
+    cases (n + 2) % 2 <;> cases bt <;> dsimp <;> rw [IH']
+
+theorem insert.correct₂ (bt : BinTree β) (n₁ n₂ : Nat) (x : β) : n₁ ≠ n₂ → get? (insert bt n₁ x) n₂ = get? bt n₂ := by
+  revert bt n₁;
+  let motive := fun n₂ => ∀ (bt : BinTree β) (n₁ : Nat), n₁ ≠ n₂ →
+    get? (insert bt n₁ x) n₂ = get? bt n₂
+  apply Bin.induction (motive:=motive)
+  case base₀ => intros bt n₂ _; cases bt <;> rfl
+  case base₁ =>
+    intros bt n₂ contra;
+    match n₂ with
+    | 0 => rfl
+    | 1 => contradiction
+    | n₂ + 2 => rw [insert.succSucc]; cases (n₂ + 2) % 2 <;> cases bt <;> rfl
+  case ind =>
+    intros n₂ IH bt n₁ hne;
+    rw [get?.succSucc bt, get?.succSucc (insert bt n₁ x)]
+    match n₁ with
+    | 0 => cases bt <;> rfl
+    | 1 => cases bt <;> rfl
+    | n₁ + 2 =>
+      rw [insert.succSucc, left!, right!]
+      have hne' : (n₁ + 2) % 2 = (n₂ + 2) % 2 → (n₁ + 2) / 2 ≠ (n₂ + 2) / 2 := by
+        intro heq h; apply hne;
+        rw [← Nat.div_add_mod (n₁ + 2) 2, ← Nat.div_add_mod (n₂ + 2) 2]
+        rw [heq, h]
+      have hmod : ∀ {n n'}, (n % 2) = .succ n' → n % 2 = 1 := by
+        intros n n' H;
+        have hle : (n % 2) < 2 := Nat.mod_lt _ (.step .refl)
+        revert H hle; cases (n % 2)
+        case zero => intro contra; cases contra
+        case succ a =>
+          intro H hle; cases a
+          case zero => rfl
+          case succ a =>
+            let u := fun {n m} => @Nat.le_of_succ_le_succ n m
+            have hle' := u (u hle); cases hle'
+      cases h₂ : (n₂ + 2) % 2 <;> cases h₁ : (n₁ + 2) % 2 <;> cases bt <;> dsimp <;> try rfl
+      case zero.zero.leaf =>
+        rw [IH _ _ (hne' (.trans h₁ (.symm h₂)))]; rfl;
+      case zero.zero.node =>
+        rw [IH _ _ (hne' (.trans h₁ (.symm h₂)))]; rfl;
+      case succ.succ.leaf =>
+        rw [IH _ _ (hne' (.trans (hmod h₁) (.symm (hmod h₂))))]; rfl;
+      case succ.succ.node =>
+        rw [IH _ _ (hne' (.trans (hmod h₁) (.symm (hmod h₂))))]; rfl;
+
+end BinTree
     
-structure QList (α : Sort _) where
-  data : BinTree α
-  size : Nat
-  default : α
+structure BinList (α : Sort _) where
+  head : Option α
+  tail : BinTree α
+
+namespace BinList
+
+def get? (bl : BinList α) (n : Nat) : Option α :=
+  match n with
+  | 0 => bl.head
+  | n => bl.tail.get? n
+
+end BinList
+
+end Auto
