Auto/Embedding/LCtx.lean
@@ -1,11 +1,12 @@
 import Auto.Lib.HEqExtra
-import Std.Data.Nat.Lemmas
+import Auto.Lib.NatExtra
+import Auto.Lib.BoolExtra
 import Std.Data.List.Lemmas
 
 namespace Auto.Embedding
 
 
-section list
+section hlist
 
   inductive HList (β : α → Sort _) : List α → Sort _
     | nil  : HList β .nil
@@ -17,52 +18,7 @@ section list
     | .(_), .cons a _,  0       => a
     | .(_), .cons _ as, .succ n => HList.getD default as n
 
-end list
-
-
-section lem
-  
-  theorem Nat.lt_of_ble_eq_false {n : Nat} : Nat.ble n pos = false → pos < n := by
-    intro H; apply Nat.lt_of_not_le;
-    intro hle; rw [Nat.ble_eq_true_of_le hle] at H; cases H
-  
-  theorem Nat.ble_eq_false_of_lt (n : Nat) : pos < n → Nat.ble n pos = false := by
-    intro H;
-    cases h₁ : Nat.ble n pos
-    case false => rfl
-    case true =>
-      simp at h₁;
-      have h₂ := Nat.not_le_of_lt H
-      apply False.elim (h₂ h₁)
-  
-  theorem Nat.ble_eq_false_eq_lt (n : Nat) : (pos < n) = (Nat.ble n pos = false) := by
-    apply propext; apply Iff.intro
-    case a.mp => apply Nat.ble_eq_false_of_lt
-    case a.mpr => apply Nat.lt_of_ble_eq_false
-
-  theorem Nat.ble_add (a b e : Nat) : Nat.ble a b = Nat.ble (a + e) (b + e) := by
-    induction e
-    case zero => rfl
-    case succ e => rw [e]; rfl
-
-  theorem Nat.eq_of_le_of_lt_succ {n m : Nat} (h₁ : n ≤ m) (h₂ : m < n + 1) : m = n :=
-    Nat.le_antisymm (Nat.le_of_succ_le_succ h₂) h₁
-
-  theorem Nat.one_add (n : Nat) : 1 + n = Nat.succ n := by simp [Nat.add_comm]
-
-  theorem Nat.pred_sub (n m : Nat) : Nat.pred n - m = Nat.pred (n - m) := by
-    rw [← Nat.sub_one, Nat.sub_sub, one_add, Nat.sub_succ]
-
-  theorem Bool.eq_false_of_ne_true {a : Bool} : a ≠ true → a = false := by
-    cases a <;> decide
-
-  theorem Bool.ne_true_of_eq_false {a : Bool} : a = false → a ≠ true := by
-    cases a <;> decide
-
-  theorem Bool.eq_false_eq_not_eq_true {a : Bool} : (a ≠ true) = (a = false) := by
-    cases a <;> decide    
-  
-end lem
+end hlist
 
 
 section generic
