Auto/Lib/NatExtra.lean
@@ -1,0 +1,36 @@
+import Std.Data.Nat.Lemmas
+
+namespace Auto
+
+theorem Nat.lt_of_ble_eq_false {n : Nat} : Nat.ble n pos = false → pos < n := by
+  intro H; apply Nat.lt_of_not_le;
+  intro hle; rw [Nat.ble_eq_true_of_le hle] at H; cases H
+
+theorem Nat.ble_eq_false_of_lt (n : Nat) : pos < n → Nat.ble n pos = false := by
+  intro H;
+  cases h₁ : Nat.ble n pos
+  case false => rfl
+  case true =>
+    simp at h₁;
+    have h₂ := Nat.not_le_of_lt H
+    apply False.elim (h₂ h₁)
+
+theorem Nat.ble_eq_false_eq_lt (n : Nat) : (pos < n) = (Nat.ble n pos = false) := by
+  apply propext; apply Iff.intro
+  case a.mp => apply Nat.ble_eq_false_of_lt
+  case a.mpr => apply Nat.lt_of_ble_eq_false
+
+theorem Nat.ble_add (a b e : Nat) : Nat.ble a b = Nat.ble (a + e) (b + e) := by
+  induction e
+  case zero => rfl
+  case succ e => rw [e]; rfl
+
+theorem Nat.eq_of_le_of_lt_succ {n m : Nat} (h₁ : n ≤ m) (h₂ : m < n + 1) : m = n :=
+  Nat.le_antisymm (Nat.le_of_succ_le_succ h₂) h₁
+
+theorem Nat.one_add (n : Nat) : 1 + n = Nat.succ n := by simp [Nat.add_comm]
+
+theorem Nat.pred_sub (n m : Nat) : Nat.pred n - m = Nat.pred (n - m) := by
+  rw [← Nat.sub_one, Nat.sub_sub, one_add, Nat.sub_succ]
+
+end Auto
